begin kmp

Part 2 - Dafny/grep-kmp/grep.dfy
@@ -7,8 +7,144 @@
 
 include "Io.dfy"
 
+
+predicate inRange(i: int, len: int, j: int, len2: int) {
+  0 <= i < len && 0 <= j < len2
+}
+
+method fillLps(query: array<char>) returns (lps: array<int>)
+requires query.Length > 0
+{
+  lps := new int[query.Length];
+  var len := 0;
+  var i := 1;
+  lps[0] := 0;
+
+  while(i < query.Length)
+  invariant i <= query.Length
+  decreases query.Length - i
+  {
+    if(query[i] == query[len]){
+      len := len + 1;
+      lps[i] := len;
+      i := i + 1;
+    } else {
+      if(len != 0){
+        len := lps[len - 1];
+      } 
+        else {
+          lps[i] := len;
+          i := i + 1;
+      }
+    }
+
+  }
+}
+
+
+method Grep(word: array<byte>, query: array<char>) returns (found: bool, pos: int)
+requires word.Length > 0
+requires query.Length > 0
+{
+  var lps := fillLps(query);
+  var indexQuery, indexWord := 0, 0;
+  while(indexWord< word.Length)
+  decreases word.Length - indexWord
+  {
+    if(indexQuery < query.Length && indexWord < word.Length && query[indexQuery] == word[indexWord] as char){
+      indexWord := indexWord+1;
+      indexQuery := indexQuery+1;
+    }
+    if(indexQuery == query.Length){
+      return true,indexWord-indexQuery;
+    } else if(indexQuery < query.Length && indexWord < word.Length && query[indexQuery] != word[indexWord] as char){
+      if(indexQuery != 0 && indexQuery < lps.Length){
+        indexQuery := lps[indexQuery -1];  
+      } else{
+        indexWord := indexWord +1;
+      }
+    }
+  }
+
+
+}
+
 method {:main} Main(ghost env:HostEnvironment?)
   requires env != null && env.Valid() && env.ok.ok();
+  modifies env.ok
+  modifies env.files
 {
-  print "TODO!\n";  
+  var ncmd := HostConstants.NumCommandLineArgs(env);
+
+    if ncmd != 3 {
+      if ncmd >= 1 {
+        print ncmd - 1; print " files supplied.\n";
+      }
+      print "Command requires stringQuery and file... Example: ./grep.exe Query File";
+      return;
+    }
+
+    var query := HostConstants.GetCommandLineArg(1, env);
+    var srcFile := HostConstants.GetCommandLineArg(2, env);
+    var ok;
+
+    ok := FileStream.FileExists(srcFile, env);
+
+    if !ok {
+      print "In file '"; print srcFile; print "'doesn't exist";
+      return;
+    }
+
+    var len;
+
+    ok, len := FileStream.FileLength(srcFile, env);
+
+    if !ok {
+      print "Couldn't stat file '"; print srcFile; print "' length";
+      return;
+    }
+    
+    var fs;
+
+    ok, fs := FileStream.Open(srcFile, env);
+    
+    if !ok {
+      print "Problems opening file "; print srcFile; print "\n";
+      return;
+    }
+
+    var buffer := new byte[len];
+    ok := fs.Read(0, buffer, 0, len);
+
+    if !ok {
+      print "Problems reading in file'"; print srcFile; print "'\n";
+      return;
+    }
+
+    var i := buffer.Length;
+
+    ok := fs.Close();
+
+    if !ok {
+      print "Problems closing in file '"; print srcFile; print "'\n";
+      return;
+    }
+
+    if buffer.Length == 0 {
+      print "File is empty, exiting.";
+      return;
+    }
+    if query.Length == 0 {
+      print "Empty query, exiting.";
+      return;
+    }
+
+    var found, pos:= Grep(buffer, query);
+    
+    if found {
+     print "YES",", ", pos;
+    }
+    else {
+      print "NO";
+    }
 }
